theories/executable.v
@@ -1,0 +1,20 @@
+From Equations Require Import Equations.
+Require Import Autosubst2.core Autosubst2.fintype Autosubst2.syntax
+  common typing preservation admissible fp_red structural soundness.
+Require Import algorithmic.
+From stdpp Require Import relations (rtc(..), nsteps(..)).
+Require Import ssreflect ssrbool.
+
+Definition metric {n} k (a b : PTm n) :=
+  exists i j va vb, nsteps LoRed.R i a va /\ nsteps LoRed.R j b vb /\
+  nf va /\ nf vb /\ size_PTm va + size_PTm vb + i + j <= k.
+
+Search (nat -> nat -> bool).
+
+Equations check_equal {n k} (a b : PTm n) (h : metric k a b) :
+  bool by wf k lt :=
+  check_equal (PAbs a) (PAbs b) h := check_equal a b _;
+  check_equal (PPair a0 b0) (PPair a1 b1) h :=
+    check_equal a0 b0 _ && check_equal a1 b1 _;
+  check_equal (PUniv i) (PUniv j) _ := _;
+  check_equal _ _ _ := _.
